Translation/Entry.lean
@@ -5,12 +5,10 @@ import Translation.Ty
 import Translation.Term
 
 
-def Surface.Entry.translate : Surface.Entry -> Core.Entry
-| data x K ctors => .data x K.translate ((λ x => (x.1 , x.2.translate)) <$>ctors)
-| ctor x i T => .ctor x i T.translate
-| opent x K => .opent x K.translate
-| openm x T => .openm x T.translate
-| instty x T => .instty x T.translate
-| defn x T t =>  sorry
+-- def Surface.Entry.translate : Surface.Entry -> Core.Entry
+-- | data x K ctors => .data x K.translate ((λ x => (x.1 , x.2.translate)) <$>ctors)
+-- | ctor x i T => .ctor x i T.translate
+-- | openm x T ms => .openm x T.translate
+-- | defn x T t =>  sorry
 
-notation "⟦" e "⟧" => Surface.Entry.translate e
+-- notation "⟦" e "⟧" => Surface.Entry.translate e
