Translation/Global.lean
@@ -6,37 +6,54 @@ import Surface.Typing
 import Translation.Ty
 import Translation.Term
 
+
+
+
+
+
 def Surface.Ty.translate_ctors (ctors : Vect n (String × Surface.Ty)) : (Vect n (String × Core.Ty)) :=
   (λ (x, ty) => (x , ty.translate)) <$> ctors
 
 
-@[simp]
-def Surface.Global.translate (G : Surface.GlobalEnv) (G' : Core.GlobalEnv) : Global -> Option Core.Global
-| .data (n := n) x K ctors =>
-  let ctors' := Ty.translate_ctors ctors
-  Core.Global.data n x K.translate ctors'
-| instty x K => return .instty x K.translate
-| inst x t => do
-  let T <- Surface.lookup_type G x
-  let t' <- t.type_chk_translate G G' [] [] T
-  return .inst x t'
-| defn x T t => do
-  let t' <- t.type_chk_translate G G' [] [] T
-  return .defn x T.translate t'
-| openm x T => return .openm x T.translate
-| opent x K => return .opent x K.translate
+-- @[simp]
+-- def Surface.Global.translate (G : Surface.GlobalEnv) (G' : Core.GlobalEnv) : Global -> Option Core.Global
+-- | .data (n := n) x K ctors =>
+--   let ctors' := Ty.translate_ctors ctors
+--   Core.Global.data n x K.translate ctors'
+-- | instDecl x t => do
+--   let T <- Surface.lookup_type G x
+--   let t' <- t.type_chk_translate G G' [] [] T
+--   return .inst x t'
+-- | defn x T t => do
+--   let t' <- t.type_chk_translate G G' [] [] T
+--   return .defn x T.translate t'
+-- | openm x T => return .openm x T.translate
+-- | opent x K => return .opent x K.translate
 
 
-@[simp]
-def Surface.GlobalEnv.translate : Surface.GlobalEnv -> Option (Core.GlobalEnv)
-| [] => return []
-| .cons g gs => do
-  let gs' <- Surface.GlobalEnv.translate gs
-  let g' <- g.translate gs gs'
-  return (g' :: gs')
+
+-- @[simp]
+-- def Surface.GlobalEnv.translate : Surface.GlobalEnv -> Option (Core.GlobalEnv)
+-- | [] => return []
+-- | .cons g gs => do
+--   let gs' <- Surface.GlobalEnv.translate gs
+--   let g' <- g.translate gs gs'
+--   return (g' :: gs')
 
 -- def Surface.Entry.translate : Surface.Entry -> Option
 
+inductive Surface.Global.Elab : Surface.GlobalEnv -> Core.GlobalEnv -> Prop
+| nil : Surface.Global.Elab [] []
+| defn :
+  Surface.Global.Elab G G' ->
+  Surface.Term.Elab G G' .chk [] [] t T t' ->
+  Surface.Global.Elab (.cons (.defn x T t) G) ((.defn x (T.translate) t') :: G')
+| data {n : Nat} {ctors : Vect n (String × Ty)} {ctors' : Vect n (String × Core.Ty)} :
+  Surface.Global.Elab G G' ->
+  ctors' = (λ i => ((ctors i).1 , (ctors i).2.translate)) ->
+  Surface.Global.Elab (.cons (.data (n := n) x K ctors) G) (.cons (.data n x K.translate ctors') G')
+
+notation:170 G:170 " -↪ " G':170 => Surface.Global.Elab G G'
 
 namespace Test.Core.Global
 
