Translation/Examples/Boolean.lean
@@ -43,8 +43,8 @@ def Surface.eqBool : Term := λˢ[ .global "Bool" ] λˢ[ .global "Bool" ]
 
 
 -- #eval Surface.BoolCtx.infer
-#eval! Surface.GlobalEnv.translate Surface.BoolCtx
+-- #eval! Surface.GlobalEnv.translate Surface.BoolCtx
 
-#eval! do let gs' : Core.GlobalEnv <- Surface.BoolCtx.translate
-          let t' <- Surface.eqBool.translate gs' [] []
-          return t'
+-- #eval! do let gs' : Core.GlobalEnv <- Surface.BoolCtx.translate
+--           let t' <- Surface.eqBool.translate gs' [] []
+--           return t'
