Translation/Global/Lemmas.lean
@@ -7,74 +7,106 @@ import Core.Typing
 import Translation.Ty.Lemmas
 import Translation.Term.Lemmas
 import Translation.Global
+import Core.Metatheory.Determined.Semantic
+-- theorem Translation.Ty.ValidCtor :
+--   Surface.ValidCtor x T -> Core.ValidCtor x ⟦T⟧ := by
+-- intro h; induction h <;> simp at *
+-- case base h1 h2 =>
+--   replace lem := Translation.Ty.Spine h2 rfl
+--   rcases lem with ⟨_, lem⟩
+--   constructor; assumption
+-- case all ih => apply Core.ValidCtor.all ih
+-- case arrow ih => apply Core.ValidCtor.arrow ih
 
-theorem Translation.Ty.ValidCtor :
-  Surface.ValidCtor x T -> Core.ValidCtor x ⟦T⟧ := by
-intro h; induction h <;> simp at *
-case base h1 h2 =>
-  replace lem := Translation.Ty.Spine h2 rfl
-  rcases lem with ⟨_, lem⟩
-  constructor; assumption
-case all ih => apply Core.ValidCtor.all ih
-case arrow ih => apply Core.ValidCtor.arrow ih
+-- theorem Translation.Global.empty_data_wkn {G : Surface.GlobalEnv} {G' : Core.GlobalEnv} (x : String) (K : Surface.Kind) :
+--   G.translate = G' ->
+--   Surface.GlobalEnv.translate (.data x K Vect.nil :: G) = (.data 0 x ⟦K⟧ Vect.nil :: G') := by
+-- intro h; simp [Surface.GlobalEnv.translate]; exact h
 
-theorem Translation.Global.empty_data_wkn {G : Surface.GlobalEnv} {G' : Core.GlobalEnv} (x : String) (K : Surface.Kind) :
-  G.translate = G' ->
-  Surface.GlobalEnv.translate (.data x K Vect.nil :: G) = (.data 0 x ⟦K⟧ Vect.nil :: G') := by
-intro h; simp [Surface.GlobalEnv.translate]; exact h
+-- theorem Surface.GlobalEnvWf.empty_data_wkn x K :
+--   ⊢s G -> lookup x G = none ->
+--   ⊢s (Surface.Global.data x K Vect.nil :: G) := by
+--  intro wf lk; apply ListGlobalWf.cons
+--  · apply GlobalWf.data <;> try simp at *
+--    apply Vect.nil
+--    apply lk
+--  · assumption
 
-theorem Surface.GlobalEnvWf.empty_data_wkn x K :
-  ⊢s G -> lookup x G = none ->
-  ⊢s (Surface.Global.data x K Vect.nil :: G) := by
- intro wf lk; apply ListGlobalWf.cons
- · apply GlobalWf.data <;> try simp at *
-   apply Vect.nil
-   apply lk
- · assumption
+-- theorem Translation.GlobalWf.sound {G : Surface.GlobalEnv} {g : Surface.Global}:
+--   ⊢s G ->
+--   Surface.GlobalWf G g ->
+--   G.translate = G' ->
+--   ⊢ G' ->
+--  ∃ g',
+--     g.translate = g'  ∧
+--     Core.GlobalWf G' g' := by
+-- intro wf h1 h2 h3; induction g <;> simp at *
+-- cases h1
+-- case _ n x K ctors cns lk cnsdef ctor_trans =>
+-- let ctors' : Vect n (String × Core.Ty) := Surface.Ty.translate_ctors ctors
+-- apply Core.GlobalWf.data
+-- · intro i y T e;
+--   replace ctor_trans := ctor_trans i (ctors i).fst (ctors i).snd rfl;
+--   rcases ctor_trans with ⟨k1, k2, k3, k4⟩
+--   rcases e with ⟨e1, e2⟩;
+--   have lemG := Translation.Global.empty_data_wkn x K h2
+--   have wfG := Surface.GlobalEnvWf.empty_data_wkn x K wf lk
+--   have lem := Translation.Ty.sound wfG (G := .data x K Vect.nil :: G) ⟨k1,lemG, rfl⟩
+--   apply And.intro
+--   · rcases lem with ⟨K', T', e1, e2, e3⟩;
+--     simp at e1; subst e1; subst e2; simp [Surface.KindEnv.translate] at e3; apply e3
+--   · apply And.intro
+--     · apply Translation.Ty.ValidCtor k2
+--     · apply And.intro; assumption
+--       apply Translation.GlobalEnv.lookup_none_sound _ h2 k4
+-- · assumption
+-- · apply Translation.GlobalEnv.lookup_none_sound _ h2 lk
 
-theorem Translation.GlobalWf.sound {G : Surface.GlobalEnv} {g : Surface.Global}:
+
+-- theorem Translation.GlobalEnv.wf_sound {G : Surface.GlobalEnv} :
+--   ⊢s G ->
+--   ⊢ G.translate
+-- := by
+-- intro wf
+-- induction G <;> simp at *
+-- case _ => apply Core.ListGlobalWf.nil
+-- case _ g gs ih =>
+-- cases wf; case _ wfgs wfg =>
+-- replace ih := ih wfgs
+-- have lem := Translation.GlobalWf.sound wfgs  wfg rfl ih
+-- rcases lem with ⟨g', lem1, lem2⟩; subst g'
+-- cases g; simp [Surface.Global.translate] at lem2;
+-- apply Core.ListGlobalWf.cons _ ih
+-- simp; apply lem2
+
+
+theorem Surface.Global.Elab.sound :
   ⊢s G ->
-  Surface.GlobalWf G g ->
-  G.translate = G' ->
-  ⊢ G' ->
- ∃ g',
-    g.translate = g'  ∧
-    Core.GlobalWf G' g' := by
-intro wf h1 h2 h3; induction g <;> simp at *
-cases h1
-case _ n x K ctors cns lk cnsdef ctor_trans =>
-let ctors' : Vect n (String × Core.Ty) := Surface.Ty.translate_ctors ctors
-apply Core.GlobalWf.data
-· intro i y T e;
-  replace ctor_trans := ctor_trans i (ctors i).fst (ctors i).snd rfl;
-  rcases ctor_trans with ⟨k1, k2, k3, k4⟩
-  rcases e with ⟨e1, e2⟩;
-  have lemG := Translation.Global.empty_data_wkn x K h2
-  have wfG := Surface.GlobalEnvWf.empty_data_wkn x K wf lk
-  have lem := Translation.Ty.sound wfG (G := .data x K Vect.nil :: G) ⟨k1,lemG, rfl⟩
+  G -↪ G' ->
+  ⊢ G' ∧ Core.Global.Determined G' := by
+intro wf h
+induction h
+case nil =>
   apply And.intro
-  · rcases lem with ⟨K', T', e1, e2, e3⟩;
-    simp at e1; subst e1; subst e2; simp [Surface.KindEnv.translate] at e3; apply e3
-  · apply And.intro
-    · apply Translation.Ty.ValidCtor k2
-    · apply And.intro; assumption
-      apply Translation.GlobalEnv.lookup_none_sound _ h2 k4
-· assumption
-· apply Translation.GlobalEnv.lookup_none_sound _ h2 lk
-
-
-theorem Translation.GlobalEnv.wf_sound {G : Surface.GlobalEnv} :
-  ⊢s G ->
-  ⊢ G.translate
-:= by
-intro wf
-induction G <;> simp at *
-case _ => apply Core.ListGlobalWf.nil
-case _ g gs ih =>
-cases wf; case _ wfgs wfg =>
-replace ih := ih wfgs
-have lem := Translation.GlobalWf.sound wfgs  wfg rfl ih
-rcases lem with ⟨g', lem1, lem2⟩; subst g'
-cases g; simp [Surface.Global.translate] at lem2;
-apply Core.ListGlobalWf.cons _ ih
-simp; apply lem2
+  · apply Core.ListGlobalWf.nil;
+  · simp [Core.Global.Determined, Core.Determined.openm, Core.Determined.defn, Core.lookup];
+case defn t T t' x j0 jdef ih =>
+  cases wf; case _ wfh wftl =>
+  replace ih := ih wfh
+  cases wftl; case _ lk j1 j2 =>
+  replace j1 := Translation.Ty.sound j1 j0 rfl
+  rcases j1 with ⟨K, T', e1, e2, j1⟩
+  subst e1; cases e2; simp at j1;
+  replace j2 := Translation.Term.Sound2 j0 jdef [] [] rfl rfl
+  apply And.intro
+  · apply Core.ListGlobalWf.cons _ ih.1
+    apply Core.GlobalWf.defn j1 j2.2
+    · apply Translation.GlobalEnv.lookup_none_sound x j0 lk
+  · sorry
+case data wf =>
+  sorry
+  -- apply Core.ListGlobalWf.cons _ wf
+  -- apply Core.GlobalWf.data
+  -- sorry
+  -- sorry
+  -- sorry
